src/Analysis/Instances/Sign/Sign_Exec.thy
@@ -193,7 +193,7 @@ proof (rule apply_tf_wrap_eqI[
   show "\<And>c. fun_of_resolved_st_q_for gs
       (sign_tf_st_for gs (EA_Check c) s) =
     apply_tf (sign_tf_for gs) (EA_Check c) (fun_of_resolved_st_q_for gs s)"
-    by simp
+    by (simp add: sign_tf_for_def event_sign_def)
 qed
 
 lemma enter_frame_sign_st_for_commute:
